Begin to build a class hierarchy in Loops.lean
That is, instead of having 'SimpleLoopState' as the only class, now
we have LoopBase, LoopForward, and LoopIncI32. LoopBase includes
the termination proof and proofs of certain invariants. LoopForward
adds a 'TerminationParam' that must always increase up to some bound.
LoopInc32 uses a 32-bit integer for the termination parameter and
always increments that parameter by a constant amount.

This change also replaces the original 'SimpleLoopState' in Primes.lean
with LoopInc32.

TODO: The termination condition used in LoopIncI32 doesn't match
the termination condition in LoopBase (being the negation of a Bool)
so some of the theorems on the base class are awkward to apply to
LoopIncI32. This should be fixed.

FormalVerifyMisc/CodeChef/Template/Primes.lean
@@ -214,7 +214,7 @@ theorem mark_multiples_state_size_pos (MMS : MarkMultiplesState) : 0 < MMS.A.siz
 /- When adding 'inc' to 'cur' we can move the addition across the 'toInt' conversion
 
   Note: We would like to use 'simple_loop_state_toInt_cur_add_inc' instead, but we
-  can only use that once we prove 'MarkMultiplesState' is a 'SimpleLoopState', but
+  can only use that once we prove 'MarkMultiplesState' is a 'LoopIncI32', but
   we need this result in order to prove that.
 -/
 lemma mms_cur_add_inc_toInt
@@ -275,7 +275,7 @@ lemma int32_lt_ofNat_iff_toInt_natAbs_lt {a : Int32} {n : ℕ}
   rw [Int32.toInt_ofNat_of_lt hlt]
   rw [Int.ofNat_natAbs_of_nonneg hnn]
 
--- The SimpleLoopState needs the upper bound of the loop stated as an Int32
+-- The LoopIncI32 needs the upper bound of the loop stated as an Int32
 -- while the MarkMultipleState has it as a natural number. This lemma
 -- allows us to convert between the two
 lemma mark_multiples_state_size_ofNat_toInt (MMS : MarkMultiplesState) :
@@ -287,7 +287,7 @@ lemma mark_multiples_state_cur_lt_size_iff (MMS : MarkMultiplesState) :
   MMS.cur < Int32.ofNat MMS.A.size ↔ MMS.cur.toInt.natAbs < MMS.A.size :=
   int32_lt_ofNat_iff_toInt_natAbs_lt (le_of_lt MMS.curpos) (lt_trans MMS.hAslt (by simp))
 
-instance : SimpleLoopState MarkMultiplesState where
+instance : LoopIncI32 MarkMultiplesState where
   cur := MarkMultiplesState.cur
   inc := MarkMultiplesState.inc
   finish := fun mms ↦ Int32.ofNat mms.A.size
@@ -309,16 +309,16 @@ instance : SimpleLoopState MarkMultiplesState where
     simp
 
 @[simp] theorem mark_multiples_state_sls_cur (MMS : MarkMultiplesState) :
-  SimpleLoopState.cur MMS = MMS.cur := rfl
+  LoopIncI32.cur MMS = MMS.cur := rfl
 
 @[simp] theorem mark_multiples_state_sls_inc (MMS : MarkMultiplesState) :
-  SimpleLoopState.inc MMS = MMS.inc := rfl
+  LoopIncI32.inc MMS = MMS.inc := rfl
 
 @[simp] theorem mark_multiples_state_sls_finish (MMS : MarkMultiplesState) :
-  SimpleLoopState.finish MMS = Int32.ofNat MMS.A.size := rfl
+  LoopIncI32.finish MMS = Int32.ofNat MMS.A.size := rfl
 
 @[simp] theorem mark_multiples_state_sls_adv (MMS : MarkMultiplesState) :
-  SimpleLoopState.adv MMS = fun hlt ↦
+  LoopIncI32.adv MMS = fun hlt ↦
   mark_multiples_advance MMS (by
     simp at hlt
     exact ((mark_multiples_state_cur_lt_size_iff MMS).mp hlt)
@@ -418,26 +418,26 @@ theorem mark_multiples_advance_changed (MMS : MarkMultiplesState)
 -/
 def mark_multiples {L : ℕ} (A : Array Int32)
   (hsize : A.size = L) (args : MMSArgs L) : MarkMultiplesState :=
-  do_simple_loop (mark_multiples_state_of_sieve A hsize args)
+  do_loop (mark_multiples_state_of_sieve A hsize args)
 
 -- The size of the marked array is the same as the size of the sieve
 @[simp] theorem mark_multiples_size {L : ℕ} (S : Sieve L) :
   (mark_multiples S.divs S.hsize (mms_args_of_sieve S)).A.size = S.divs.size := by
   unfold mark_multiples
   rw [← mark_multiples_state_of_sieve_size S]
-  apply simple_loop_val_const (_ : MarkMultiplesState) (fun mms ↦ mms.A.size)
+  apply loop_val_const (_ : MarkMultiplesState) (fun mms ↦ mms.A.size)
   intro mms hlt
   apply mark_multiples_advance_size mms
 
 -- The increment of the marked array is the same as S.i
 @[simp] theorem mark_multiples_inc {L : ℕ} (S : Sieve L) :
   (mark_multiples S.divs S.hsize (mms_args_of_sieve S)).inc = S.i :=
-  @simple_loop_inc_const MarkMultiplesState _ _
+  @loop_incI32_inc_const MarkMultiplesState _ _
 
 -- Prove the equivalence between cur < finish in the SimpleLoopState interface
 -- and the corresponding statement in MarkMultiplesState
 lemma mark_multiples_cur_lt_size_iff_cur_lt_finish (MMS : MarkMultiplesState) :
-  MMS.cur.toInt.natAbs < MMS.A.size ↔ SimpleLoopState.cur MMS < SimpleLoopState.finish MMS := by
+  MMS.cur.toInt.natAbs < MMS.A.size ↔ LoopIncI32.cur MMS < LoopIncI32.finish MMS := by
   rw [← mark_multiples_state_cur_lt_size_iff MMS]; simp
 
 -- 'mark_multiples' has no effect on entries in the sieve
@@ -456,7 +456,7 @@ theorem mark_multiples_unchanged_of_marked {L : ℕ} (S : Sieve L) :
     unfold prop mms₀
     intro; simpa
   have step : ∀ t curlt,
-    prop t → prop (SimpleLoopState.adv t curlt) := by
+    prop t → prop (LoopIncI32.adv t curlt) := by
     unfold prop
     intro t curlt h jlt'; simp
     rw [← mark_multiples_cur_lt_size_iff_cur_lt_finish] at curlt
@@ -464,7 +464,10 @@ theorem mark_multiples_unchanged_of_marked {L : ℕ} (S : Sieve L) :
     obtain ⟨hnz', h⟩ := h jlt'
     rw [mark_multiples_advance_unchanged_of_marked t curlt j jpos jlt' hnz']
     exact ⟨hnz', h⟩
-  exact (simple_loop_prop_const mms₀ prop base step _).2
+  apply (loop_prop_const mms₀ prop base _ _).2
+  intro t hterm hpt
+  simp only [LoopBase.term, decide_eq_true_eq] at hterm
+  exact step t (Int32.not_le.mp hterm) hpt
 
 -- 'mark_multiples' has no effect on entries in the sieve
 -- whose indices are not divisible by 'inc'
@@ -481,7 +484,7 @@ theorem mark_multiples_unchanged_of_not_dvd {L : ℕ} (S : Sieve L) :
     unfold prop mms₀
     intro; simpa
   have step : ∀ t curlt,
-    prop t → prop (SimpleLoopState.adv t curlt) := by
+    prop t → prop (LoopIncI32.adv t curlt) := by
     unfold prop
     intro t curlt h jlt'; simp
     rw [← mark_multiples_cur_lt_size_iff_cur_lt_finish] at curlt
@@ -489,7 +492,10 @@ theorem mark_multiples_unchanged_of_not_dvd {L : ℕ} (S : Sieve L) :
     obtain ⟨hdvd', h⟩ := h jlt'
     rw [mark_multiples_advance_unchanged_of_not_dvd t curlt j jpos jlt' hdvd']
     exact ⟨hdvd', h⟩
-  exact (simple_loop_prop_const mms₀ prop base step _).2
+  apply (loop_prop_const mms₀ prop base _ _).2
+  intro t hterm hpt
+  simp only [LoopBase.term, decide_eq_true_eq] at hterm
+  exact step t (Int32.not_le.mp hterm) hpt
 
 -- 'mark_multiples' has no effect on the first entry in the sieve
 theorem mark_multiples_unchanged_of_first {L : ℕ} (S : Sieve L) :
@@ -503,12 +509,15 @@ theorem mark_multiples_unchanged_of_first {L : ℕ} (S : Sieve L) :
   have base : prop mms₀ := by
     unfold prop mms₀; simp
   have step : ∀ t curlt,
-    prop t → prop (SimpleLoopState.adv t curlt) := by
+    prop t → prop (LoopIncI32.adv t curlt) := by
     unfold prop
     intro t curlt h; simp
     rw [← mark_multiples_cur_lt_size_iff_cur_lt_finish] at curlt
     rwa [mark_multiples_advance_unchanged_of_first t curlt]
-  exact simple_loop_prop_const mms₀ prop base step
+  apply loop_prop_const mms₀ prop base
+  intro t hterm hpt
+  simp only [LoopBase.term, decide_eq_true_eq] at hterm
+  exact step t (Int32.not_le.mp hterm) hpt
 
 -- Any entry that was zero and has index divisible by 'inc' will be
 -- set to 'inc' by mark_multiples
@@ -531,10 +540,18 @@ theorem mark_multiples_changed {L : ℕ} (S : Sieve L) :
     intro jlt
     have lej := Int.le_of_dvd (Int.ofNat_lt_ofNat_of_lt jpos) hdvd
     exact False.elim (Int.not_lt_of_ge lej jlt)
-  have step : ∀ t curlt,
-    prop t → prop (SimpleLoopState.adv t curlt) := by
+  have step : ∀ t (hterm : ¬LoopBase.term t = true),
+    prop t → prop (LoopIncI32.adv t (by
+      simp only [LoopBase.term, decide_eq_true_eq] at hterm
+      exact Int32.not_le.mp hterm
+    )) := by
     unfold prop
     intro t curlt h jlt hinc
+    -- TODO: Currently we're working around a mismatch between
+    -- the termination definition in LoopBase and LoopIncI32
+    -- Fix the mismatch
+    simp only [LoopBase.term, decide_eq_true_eq, Int32.not_le] at curlt
+    change LoopIncI32.cur t < LoopIncI32.finish t at curlt
     simp; simp at jlt hinc
     rw [← mark_multiples_cur_lt_size_iff_cur_lt_finish] at curlt
     constructor
@@ -564,14 +581,14 @@ theorem mark_multiples_changed {L : ℕ} (S : Sieve L) :
       rw [Int.mul_le_mul_left t.incpos]
       exact Int.le_of_lt_add_one jlt'
   rw [← mark_multiples_inc]
-  have := simple_loop_prop_const mms₀ prop base step
+  have := loop_prop_const mms₀ prop base step
   apply (this _ (Int32.toInt_inj.mpr (mark_multiples_inc S))).2 _
   -- The final step is to prove that j < cur so the
   -- right-hand side of the property is applicable
   rename j < S.divs.size => jlt
   apply lt_of_lt_of_le (Int.ofNat_lt_ofNat_of_lt jlt)
-  have lecur := Int32.le_iff_toInt_le.mp (simple_loop_index_ge mms₀)
-  rw [mark_multiples_state_sls_finish] at lecur
+  have lecur : (Int32.ofNat mms₀.A.size).toInt ≤ (do_loop mms₀).cur.toInt :=
+    Int32.le_iff_toInt_le.mp (loop_forward_bound_le _ _ mms₀)
   rw [mark_multiples_state_size_ofNat_toInt] at lecur
   exact lecur
 
@@ -861,7 +878,7 @@ lemma sieve_index_lt_size_iff {L : ℕ} (S : Sieve L) :
     (by rw [S.hsize]; exact lt_trans S.hLlt (by simp))
 
 -- Prove that 'Sieve' implements a simple loop
-instance (L : ℕ) : SimpleLoopState (Sieve L) where
+instance (L : ℕ) : LoopIncI32 (Sieve L) where
   cur := Sieve.i
   inc := fun _ ↦ 1
   finish := fun S ↦ Int32.ofNat S.divs.size
@@ -879,20 +896,20 @@ instance (L : ℕ) : SimpleLoopState (Sieve L) where
   hfinish := by simp
 
 @[simp] theorem sieve_loop_cur {L : ℕ} (S : Sieve L) :
-  SimpleLoopState.cur S = S.i := rfl
+  LoopIncI32.cur S = S.i := rfl
 
 @[simp] theorem sieve_loop_inc {L : ℕ} (S : Sieve L) :
-  SimpleLoopState.inc S = 1 := rfl
+  LoopIncI32.inc S = 1 := rfl
 
 @[simp] theorem sieve_loop_finish {L : ℕ} (S : Sieve L) :
-  SimpleLoopState.finish S = Int32.ofNat S.divs.size := rfl
+  LoopIncI32.finish S = Int32.ofNat S.divs.size := rfl
 
 @[simp] theorem sieve_loop_adv {L : ℕ} (S : Sieve L) :
-  SimpleLoopState.adv S = fun hlt ↦
+  LoopIncI32.adv S = fun hlt ↦
     advance_sieve S (by rwa [← sieve_index_lt_size_iff S]) := rfl
 
 def sieve_of_eratosthenes : Sieve SIEVE_SIZE :=
-  do_simple_loop init_sieve
+  do_loop init_sieve
 
 def primes : Array Int32 := sieve_of_eratosthenes.primes
 def divs : Array Int32 := sieve_of_eratosthenes.divs
@@ -901,24 +918,32 @@ def divs : Array Int32 := sieve_of_eratosthenes.divs
 -- after loop execution is complete
 theorem sieve_of_eratosthenes_index_ge :
   SIEVE_SIZE ≤ sieve_of_eratosthenes.i.toInt := by
-  have := simple_loop_index_ge init_sieve
-  simp at this
+  have : Int32.ofNat init_sieve.divs.size ≤ (do_loop init_sieve).i :=
+    loop_forward_bound_le _ _ init_sieve
   apply Int32.le_iff_toInt_le.mp at this
   rwa [Sieve.hsize, Int32.toInt_ofNat_of_lt] at this
   unfold SIEVE_SIZE; simp
 
 theorem sieve_of_eratosthenes_index :
   sieve_of_eratosthenes.i.toInt = SIEVE_SIZE := by
-  have curlt : SimpleLoopState.cur init_sieve < SimpleLoopState.finish init_sieve := by
+  have curlt : LoopIncI32.cur init_sieve < LoopIncI32.finish init_sieve := by
     unfold init_sieve SIEVE_SIZE; simp
   apply le_antisymm _ sieve_of_eratosthenes_index_ge
   apply Int.le_of_lt_add_one
-  apply lt_of_lt_of_eq (Int32.lt_iff_toInt_lt.mp (simple_loop_index_lt_of_lt init_sieve curlt))
-  rw [simple_loop_state_toInt_finish_add_inc]
-  rw [simple_loop_finish_const, simple_loop_inc_const]; dsimp
+  have curlt' : (do_loop init_sieve).i < Int32.ofNat init_sieve.divs.size + 1 :=
+    loop_incI32_term_param_lt_of_lt init_sieve curlt
+  apply lt_of_lt_of_eq (Int32.lt_iff_toInt_lt.mp curlt')
+  have hrw :
+    (Int32.ofNat init_sieve.divs.size + 1).toInt =
+    (Int32.ofNat init_sieve.divs.size).toInt + 1 :=
+    loop_incI32_toInt_finish_add_inc init_sieve
+  rw [hrw]
   rw [Int.add_left_inj, init_sieve_size]
   apply Int32.toInt_ofNat_of_lt
   unfold SIEVE_SIZE; simp
+
+theorem primes_nonneg : ∀ n ∈ primes, 0 ≤ n :=
+  fun n nmem ↦ sieve_of_eratosthenes.hprimesnn n nmem
 
 -- The elements of 'primes' are in-fact prime
 theorem prime_of_mem_primes :
@@ -932,6 +957,14 @@ theorem prime_of_mem_primes :
   apply ((S.hpmem_iff n.toInt.natAbs).mp _).2
   rw [habs]
   exact Array.mem_map_of_mem nmem
+
+-- The elements of 'primes' are positive
+theorem primes_pos : ∀ n ∈ primes, 0 < n := by
+  intro n nmem
+  apply Int32.lt_iff_toInt_lt.mpr
+  rcases prime_of_mem_primes n nmem with ⟨p, hp, pprime⟩
+  rw [hp]
+  exact Int.ofNat_lt_ofNat_of_lt (Nat.Prime.pos pprime)
 
 -- All elements of 'primes' are less than SIEVE_SIZE
 theorem lt_of_mem_primes :
