FormalVerifyMisc/Loops.lean
@@ -1,7 +1,265 @@
 import Mathlib.Tactic.Linarith
 import FormalVerifyMisc.Int32.Basic
 
-class SimpleLoopState (α : Type) where
+-- A loop which proves termination by mapping its state to decreasing natural numbers
+class LoopBase (α : Type) where
+  -- Indicates whether the loop has reached its terminal state
+  term : α → Bool
+  -- Advance the loop, given its state is not terminal
+  adv : (s : α) → ¬term s → α
+  -- A function mapping from α to ℕ - used to prove termination
+  fdec : α → ℕ
+  -- Proof that the value of 'fdec' decreases as 'adv' is called repeatedly
+  hdec : ∀ s, (h : ¬term s) → fdec (adv s h) < fdec s
+
+def do_loop {α : Type} [LoopBase α] (s : α) :=
+  if h : LoopBase.term s then s else do_loop (LoopBase.adv s h)
+termination_by LoopBase.fdec s
+decreasing_by
+  exact LoopBase.hdec s h
+
+alias LoopReverse := LoopBase
+
+-- Loop which continues until some parameter (of type 'β') exceeds some upper bound
+-- 'β' is typically of type Int32, Int64, UInt32, or UInt64
+class LoopForward (α : Type) (β : outParam Type) [LE β] where
+  -- Upper bound for loop execution
+  bound : α → β
+  -- A map from the current loop state to β - used to check for termination
+  finc : α → β
+  -- Function for advancing the loop state
+  fadv : (s : α) → ¬bound s ≤ finc s → α
+  -- Proof that 'finc' increases as 'fadv' is called repeatedly
+  hinc : ∀ s, (h : ¬bound s ≤ finc s) → ¬finc (fadv s h) ≤ finc s
+  -- Proof that the bound doesn't change as 'fadv' is called
+  hbound : ∀ s, (h : ¬bound s ≤ finc s) → bound (fadv s h) = bound s
+
+-- A mapping from a type 'β' to the natural numbers
+-- Used in proving loop termination
+class TerminationParam (β : Type) [LE β] where
+  embed : OrderEmbedding β ℕ
+
+-- Mapping used to embed Int32 into the natural numbers
+def int32_embed_toFun (i : Int32) := (i.toInt + 2^31).natAbs
+
+-- Proves the result of embedding an Int32 into ℕ and then casting to ℤ
+lemma int32_embed_toFun_toInt (i : Int32) : (int32_embed_toFun i) = i.toInt + 2^31 := by
+  unfold int32_embed_toFun
+  rw [Int.ofNat_natAbs_of_nonneg]
+  apply Int.le_add_of_sub_right_le
+  rw [zero_sub]
+  exact int32_minval_le_toInt _
+
+-- Prove that Int32 satisfies the requirements of a termination parameter
+instance : TerminationParam Int32 where
+  embed := {
+    toFun := int32_embed_toFun
+    inj' := by
+      intro i j h
+      apply Int.ofNat_inj.mpr at h
+      rw [int32_embed_toFun_toInt, int32_embed_toFun_toInt] at h
+      rwa [Int.add_left_inj, Int32.toInt_inj] at h
+    map_rel_iff' := by
+      intro a b; dsimp
+      rw [← Int.ofNat_le]
+      rw [int32_embed_toFun_toInt, int32_embed_toFun_toInt]
+      rw [Int.add_le_add_iff_right, Int32.le_iff_toInt_le]
+  }
+
+-- Prove that a LoopForward' is also a 'LoopBase'
+instance (α β : Type)
+  [LE β] [DecidableRel (· ≤ · : β → β → Prop)]
+  [TerminationParam β] [LoopForward α β] : LoopBase α where
+  term := fun s ↦ decide (LoopForward.bound s ≤ LoopForward.finc s)
+  adv := fun s h ↦ LoopForward.fadv s (by simp at h; assumption)
+  fdec := fun s ↦
+    TerminationParam.embed (LoopForward.bound s) -
+    TerminationParam.embed (LoopForward.finc s)
+  hdec := by
+    intro s h
+    simp only [decide_eq_true_eq] at h
+    rw [LoopForward.hbound]
+    by_contra! h'
+    let embed : β ↪o ℕ := TerminationParam.embed
+    by_cases hle :
+      embed (LoopForward.finc (LoopForward.fadv s h)) ≤ embed (LoopForward.bound s)
+    · apply LoopForward.hinc s h
+      exact embed.map_rel_iff'.mp (Nat.le_of_sub_le_sub_left hle h')
+    rename' hle => hlt; push_neg at hlt
+    rw [Nat.sub_eq_zero_of_le (le_of_lt hlt)] at h'
+    have hsubzero := Nat.le_of_sub_eq_zero (Nat.eq_zero_of_le_zero h')
+    exact h (embed.map_rel_iff'.mp hsubzero)
+
+-- A loop that advances by incrementing a 32-bit integer
+class LoopIncI32 (α : Type) where
+  -- Variable to track our progress through the loop
+  cur : α → Int32
+  -- Amount by which to increment 'cur' on each iteration
+  inc : α → Int32
+  -- Upper bound for the loop
+  -- The loop will exit if 'cur' ever meets or exceeds 'finish'
+  finish : α → Int32
+  -- Function for advancing the state
+  adv : (s : α) → cur s < finish s → α
+  -- 'inc' must be positive
+  hpos : ∀ (s : α), 0 < (inc s)
+  -- A proof that the loop execution will not exceed the 32-bit limit
+  hsafe : ∀ (s : α), (finish s).toInt + (inc s).toInt ≤ Int32.maxValue.toInt
+  -- Proof that 'adv' increments 'cur' as long as 'cur' < 'finish'
+  hadv : ∀ s hlt, cur (adv s hlt) = cur s + inc s
+  -- Proof that advancing the state doesn't change 'inc'
+  hinc : ∀ s hlt, inc (adv s hlt) = inc s
+  -- Proof that advancing the state doesn't change 'finish'
+  hfinish : ∀ s hlt, finish (adv s hlt) = finish s
+
+-- 'i + inc' can be moved across the 'toInt' conversion if 'i' ≤ 'finish'
+lemma loop_incI32_toInt_val_add_inc {α : Type} [LoopIncI32 α] (s : α)
+  (i : Int32) (h : i ≤ LoopIncI32.finish s) :
+  (i + LoopIncI32.inc s).toInt =
+  i.toInt + (LoopIncI32.inc s).toInt := by
+  have incpos := Int32.lt_iff_toInt_lt.mp (LoopIncI32.hpos s)
+  apply int32_toInt_add_of_bounds
+  constructor
+  · exact Int.add_le_add (int32_minval_le_toInt _) (le_of_lt incpos)
+  · apply Int.lt_of_le_sub_one
+    rw [← Int32.toInt_maxValue]
+    apply le_trans (Int.add_le_add_right _ _) (LoopIncI32.hsafe s)
+    exact Int32.le_iff_toInt_le.mp h
+
+-- In particular, 'cur + inc' can be moved across the 'toInt' conversion
+lemma loop_incI32_toInt_cur_add_inc {α : Type} [LoopIncI32 α] (s : α)
+  (h : ¬LoopIncI32.finish s ≤ LoopIncI32.cur s) :
+  (LoopIncI32.cur s + LoopIncI32.inc s).toInt =
+  (LoopIncI32.cur s).toInt + (LoopIncI32.inc s).toInt := by
+  apply loop_incI32_toInt_val_add_inc
+  exact Int32.le_of_lt (Int32.not_le.mp h)
+
+-- In particular, 'finish + inc' can be moved across the 'toInt' conversion
+lemma loop_incI32_toInt_finish_add_inc {α : Type} [LoopIncI32 α] (s : α) :
+  (LoopIncI32.finish s + LoopIncI32.inc s).toInt =
+  (LoopIncI32.finish s).toInt + (LoopIncI32.inc s).toInt := by
+  apply loop_incI32_toInt_val_add_inc
+  exact Int32.le_refl _
+
+-- Prove that a 'LoopIncI32' is a 'LoopForward'
+instance (α : Type) [LoopIncI32 α] : LoopForward α Int32 where
+  bound := LoopIncI32.finish
+  finc := LoopIncI32.cur
+  fadv := fun s h ↦ LoopIncI32.adv s (Int32.not_le.mp h)
+  hinc := by
+    intro s h
+    rw [LoopIncI32.hadv, Int32.not_le]
+    have incpos := Int32.lt_iff_toInt_lt.mp (LoopIncI32.hpos s)
+    have := Int.add_lt_add_left incpos (LoopIncI32.cur s).toInt
+    rw [Int32.toInt_zero, add_zero] at this
+    apply Int32.lt_iff_toInt_lt.mpr
+    rwa [loop_incI32_toInt_cur_add_inc s h]
+  hbound := fun s h ↦ LoopIncI32.hfinish s (Int32.not_le.mp h)
+
+-- If a property of the loop state is constant across calls to 'adv'
+-- it will be constant over the full execution of the loop
+theorem loop_prop_const {α : Type} [LoopBase α] (s : α)
+  (prop : α → Prop) (base : prop s)
+  (step : ∀ t hlt, prop t → prop (LoopBase.adv t hlt)) :
+  prop (do_loop s) := by
+  unfold do_loop
+  split_ifs with h
+  · exact base
+  · apply loop_prop_const _ _ _ step
+    exact step s h base
+termination_by LoopBase.fdec s
+decreasing_by
+  exact LoopBase.hdec s h
+
+-- If a value in the loop state is constant across calls to 'adv'
+-- it will be constant over the full execution of the loop
+theorem loop_val_const {α β : Type} [LoopBase α] (s : α)
+  (f : α → β) (hconst : ∀ t hlt, f (LoopBase.adv t hlt) = f t) :
+  f (do_loop s) = f s := by
+  -- Prove this as a special case of 'loop_prop_const'
+  let prop : α → Prop := fun t ↦ f t = f s
+  have base : prop s := rfl
+  have step : ∀ t hlt, prop t → prop (LoopBase.adv t hlt) := by
+    intro t hlt
+    unfold prop
+    rw [hconst t hlt]
+    exact id
+  exact loop_prop_const s prop base step
+
+-- After loop execution is complete,
+-- the termination requirement has been met
+theorem loop_term {α : Type} [LoopBase α] (s : α) :
+  LoopBase.term (do_loop s) := by
+  unfold do_loop
+  split_ifs with h
+  · assumption
+  · apply loop_term
+termination_by LoopBase.fdec s
+decreasing_by
+  exact LoopBase.hdec s h
+
+-- The upper bound for a forward loop does not change over its execution
+@[simp] theorem loop_forward_bound_const (α β : Type)
+  [LE β] [DecidableRel (· ≤ · : β → β → Prop)]
+  [TerminationParam β] [LoopForward α β] (s : α) :
+  LoopForward.bound (do_loop s) = LoopForward.bound s := by
+  apply loop_val_const
+  intro t h
+  simp only [LoopBase.term, decide_eq_true_eq] at h
+  exact LoopForward.hbound t h
+
+-- After the execution of a forward loop,
+-- the termination parameter will have exceeded the bound
+theorem loop_forward_bound_le (α β : Type)
+  [LE β] [DecidableRel (· ≤ · : β → β → Prop)]
+  [TerminationParam β] [LoopForward α β] (s : α) :
+  LoopForward.bound s ≤ LoopForward.finc (do_loop s) := by
+  have := loop_term s
+  simp only [LoopBase.term, decide_eq_true_eq] at this
+  rwa [loop_forward_bound_const] at this
+
+-- 'finish' is unmodified by the loop's execution
+@[simp] theorem loop_incI32_finish_const {α : Type} [LoopIncI32 α] (s : α) :
+  LoopIncI32.finish (do_loop s) = LoopIncI32.finish s := by
+  apply loop_val_const; intros
+  apply LoopIncI32.hfinish
+
+-- 'inc' is unmodified by the loop's execution
+@[simp] theorem loop_incI32_inc_const {α : Type} [LoopIncI32 α] (s : α) :
+  LoopIncI32.inc (do_loop s) = LoopIncI32.inc s := by
+  apply loop_val_const; intros
+  apply LoopIncI32.hinc
+
+-- After loop execution, cur < finish + inc,
+-- if before loop execution cur < finish
+theorem loop_incI32_term_param_lt_of_lt {α : Type} [LoopIncI32 α] (s : α)
+  (curlt : LoopIncI32.cur s < LoopIncI32.finish s) :
+  LoopIncI32.cur (do_loop s) < LoopIncI32.finish s + LoopIncI32.inc s := by
+  have incpos := Int32.lt_iff_toInt_lt.mp (LoopIncI32.hpos s)
+  let prop (t : α) : Prop :=
+    LoopIncI32.cur t < LoopIncI32.finish t + LoopIncI32.inc t
+  have base : prop s := by
+    unfold prop
+    apply Int32.lt_iff_toInt_lt.mpr
+    rw [loop_incI32_toInt_finish_add_inc]
+    apply lt_trans (Int32.lt_iff_toInt_lt.mp curlt)
+    exact Int.lt_add_of_pos_right _ incpos
+  have step : ∀ t h, prop t → prop (LoopIncI32.adv t h) := by
+    unfold prop
+    intro t hterm curlt'
+    rw [LoopIncI32.hadv]
+    apply Int32.lt_iff_toInt_lt.mpr
+    rw [loop_incI32_toInt_finish_add_inc]
+    rw [loop_incI32_toInt_cur_add_inc _ (Int32.not_le.mpr hterm)]
+    rw [LoopIncI32.hfinish, LoopIncI32.hinc]
+    exact Int.add_lt_add_right (Int32.lt_iff_toInt_lt.mp hterm) _
+  rw [← loop_incI32_finish_const, ← loop_incI32_inc_const]
+  apply loop_prop_const _ prop base _
+  intro t hterm hpt
+  simp only [LoopBase.term, decide_eq_true_eq] at hterm
+  exact step t (Int32.not_le.mp hterm) hpt
+
+/-class SimpleLoopState (α : Type) where
   -- Variable to track our progress through the loop
   cur : α → Int32
   -- Amount by which to increment 'cur' on each iteration
@@ -183,4 +441,4 @@ theorem simple_loop_index_lt_of_lt {α : Type} [SimpleLoopState α] (s : α)
     rw [simple_loop_state_toInt_finish_add_inc]
     rw [simple_loop_state_toInt_cur_add_inc _ hlt]
     exact Int.add_lt_add_right (Int32.lt_iff_toInt_lt.mp hlt) _
-  exact simple_loop_prop_const _ prop base step
+  exact simple_loop_prop_const _ prop base step-/
